Day 2

problems/2/Problem2.dfy
@@ -1,9 +1,96 @@
+include "../../parser/split.dfy"
+include "../../parser/parseInt.dfy"
 module Problem2 {
+    import opened Split
+    import opened ParseInt
+    import opened Std.Strings
+
+    method parseInput(input: string) returns (xs: seq<(nat, nat)>)
+        ensures forall xx :: xx in xs ==> xx.0 < xx.1
+    {
+        xs := [];
+        var pairs := split(input, ",");
+        for i := 0 to |pairs| 
+            invariant forall xx :: xx in xs ==> xx.0 < xx.1
+            invariant |xs| == i
+        {
+            var pairpieces := split(pairs[i], "-");
+            expect |pairpieces| == 2;
+            var start := Integer(pairpieces[0]);
+            var end := Integer(pairpieces[1]);
+            expect 0 <= start < end;
+            xs := xs + [(start, end)];
+        }
+
+    }
+
+    function repeat(s: string, k: nat): string {
+        if k == 0 then "" else s+repeat(s, k-1)
+    }
+
+    predicate Invalid(n: string) {
+        // exists k :: 0 < k < |n| && |n| % k == 0  && n == repeat(n[..k], |n|/k)
+        // n == repeat(n[..|n|/2], 2)
+        n[..|n|/2] == n[|n|/2..]
+    }
+
+    predicate InvalidAll(n: string) {
+        exists k :: 0 < k < |n| && |n| % k == 0  && n == repeat(n[..k], |n|/k)
+        // n == repeat(n[..|n|/2], 2)
+    }
+
+    lemma testInvalid() {
+        assert Invalid("11");
+        assert Invalid("22");
+        assert Invalid("1010");
+        assert Invalid("1188511885");
+    }
+
     method problem2_1(input: string) returns (x: int) {
-        return 3;
+        var id_pairs := parseInput(input);
+        print "paiurs", id_pairs;
+        x := 0;
+        for i := 0 to |id_pairs|
+        {
+            var invalid_ids := set y | id_pairs[i].0 <= y <= id_pairs[i].1 && Invalid(OfNat(y));
+            // print "\n", id_pairs[i], " ", id_pairs[i].1-id_pairs[i].0, " ", invalid_ids;
+            ghost var all_ids := invalid_ids;
+            ghost var removed: set<int> := {};
+            while invalid_ids != {} 
+                invariant invalid_ids !! removed
+                invariant invalid_ids == all_ids - removed
+            {
+                var id :| id in invalid_ids;
+                x := x + id;
+                invalid_ids := invalid_ids - {id};
+                removed := removed+{id};
+            }
+
+        }
+        print "\n";
     }
 
     method problem2_2(input: string) returns (x: int) {
-        return 4;
+        var id_pairs := parseInput(input);
+        print "paiurs", id_pairs;
+        x := 0;
+        for i := 0 to |id_pairs|
+        {
+            var invalid_ids := set y | id_pairs[i].0 <= y <= id_pairs[i].1 && InvalidAll(OfNat(y));
+            // print "\n", id_pairs[i], " ", id_pairs[i].1-id_pairs[i].0, " ", invalid_ids;
+            ghost var all_ids := invalid_ids;
+            ghost var removed: set<int> := {};
+            while invalid_ids != {} 
+                invariant invalid_ids !! removed
+                invariant invalid_ids == all_ids - removed
+            {
+                var id :| id in invalid_ids;
+                x := x + id;
+                invalid_ids := invalid_ids - {id};
+                removed := removed+{id};
+            }
+
+        }
+        print "\n";
     }
 }
